Exclude examples/box; now it compiles

examples/mutsum/MutHeader.v
@@ -27,16 +27,16 @@ Section PROOF.
 
   Definition GlobalStb: list (fname * fspec) := [
     ("main", mk "F" (X:=unit) top3 top3) ;
-    ("f", mk "F" (X:=nat) (fun n varg _ => varg = [Vint (Z.of_nat n)]) (fun n vret _ => vret = Vint (Z.of_nat (sum n)))) ;
-    ("g", mk "F" (X:=nat) (fun n varg _ => varg = [Vint (Z.of_nat n)]) (fun n vret _ => vret = Vint (Z.of_nat (sum n))))
+    ("f", mk "F" (X:=nat) (fun n varg _ => varg = [Vint (Z.of_nat n)]↑) (fun n vret _ => vret = (Vint (Z.of_nat (sum n)))↑)) ;
+    ("g", mk "F" (X:=nat) (fun n varg _ => varg = [Vint (Z.of_nat n)]↑) (fun n vret _ => vret = (Vint (Z.of_nat (sum n)))↑))
   ].
 
 End PROOF.
 
 
-Definition ord: list val -> list val -> Prop := fun vs0 vs1 => exists n, vs0 = [Vint (Z.of_nat n)] /\ vs1 = [Vint (Z.of_nat (S n))].
+Definition _ord: list val -> list val -> Prop := fun vs0 vs1 => exists n, vs0 = [Vint (Z.of_nat n)] /\ vs1 = [Vint (Z.of_nat (S n))].
 
-Theorem ord_well_founded: well_founded ord.
+Theorem _ord_well_founded: well_founded _ord.
 Proof.
   ii. destruct a.
   { econs; ii. inv H; ss. des; clarify. }
@@ -47,4 +47,11 @@ Proof.
   pattern n. eapply well_founded_ind.
   { eapply Z.lt_wf with (z:=0%Z). }
   i. ss. econs. ii. inv H0; ss. des; clarify. eapply H. lia.
+Qed.
+
+Definition ord: Any.t -> Any.t -> Prop := fun a0 a1 => exists vs0 vs1, a0 = vs0↑ /\ a1 = vs1↑ /\ _ord vs0 vs1.
+
+Theorem ord_well_founded: well_founded ord.
+Proof.
+  admit "ez - import wf-map from CompCertM".
 Qed.
